Partial using shift

LanguagesEquivalence/L_to_Hyb.v
@@ -55,7 +55,7 @@ forall Omega Gamma w,
   Mem w Omega ->
   exists Delta,
   snd (L_to_Hyb_ctx Omega Gamma w) = Some (w, Delta).
-unfold L_to_Hyb_ctx. intros;
+unfold L_to_Hyb_ctx; intros;
 remember (bucket_sort_L Omega Gamma) as l;
 generalize dependent Omega; generalize dependent Gamma;
 generalize dependent w; induction l; intros.
@@ -253,8 +253,18 @@ inversion H0; subst;
 rewrite split_at_Hyb_snd_cons with (Delta:=Gamma_Hyb); auto.
 Qed.
 
+Lemma gather_keys_L_fresh:
+forall l w,
+  ~ Mem w (map fst l) ->
+  gather_keys_L w l = nil.
+induction l; intros; rew_map in *; simpl in *; auto.
+destruct a; case_if; simpl in *.
+elim H; apply Mem_here.
+rewrite IHl; auto; intro; elim H; rewrite Mem_cons_eq; right; auto.
+Qed.
 
-(* Term conversion *)
+
+(* Shift helpers *)
 
 (* FIXME: Move this to Hybrid/Hyb_Syntax *)
 (* ?? *)
@@ -263,7 +273,7 @@ match M with
 | hyp_Hyb v => M
 | lam_Hyb t M => lam_Hyb t (shift_term_Hyb M)
 | appl_Hyb M1 M2 => appl_Hyb (shift_term_Hyb M1) (shift_term_Hyb M2)
-| box_Hyb M => box_Hyb (shift_term_Hyb M)
+| box_Hyb M => box_Hyb (shift_term_Hyb M) (* alt: it stops here & in letdia *)
 | unbox_fetch_Hyb w M => unbox_fetch_Hyb (shift_vwo w) (shift_term_Hyb M)
 | get_here_Hyb w M => get_here_Hyb (shift_vwo w) (shift_term_Hyb M)
 | letdia_get_Hyb w M N => letdia_get_Hyb (shift_vwo w) (shift_term_Hyb M)
@@ -271,22 +281,14 @@ match M with
 end.
 
 (* FIXME: Move this to Hybrid/Hyb_Substitution *)
-Lemma shift_vwo_shift_term_Hyb:
-forall M w0 w1,
-  {{shift_vwo w0 // shift_vwo w1}} (shift_term_Hyb M) =
-  shift_term_Hyb ({{w0 // w1}} M).
-induction M; intros; simpl in *; auto;
-try (rewrite IHM; eauto);
-try (rewrite IHM1; try rewrite IHM2; eauto);
-repeat case_if; auto; try destruct v; try destruct w1; simpl in *;
-inversion H; subst; elim H0; auto.
-Qed.
-
-(* FIXME: Move this to Hybrid/Hyb_Substitution *)
 Lemma lc_w_n_shift_term_Sn_Hyb:
 forall N n,
-  lc_w_n_Hyb (S n) (shift_term_Hyb N) ->
+  lc_w_n_Hyb (S n) (shift_term_Hyb N) <->
   lc_w_n_Hyb n N.
+split; generalize dependent n; generalize dependent N.
+induction N; intros; inversion H; subst; simpl in *; unfold shift_vwo in *;
+try (destruct v; inversion H0; subst);
+constructor; auto; omega.
 induction N; intros; inversion H; subst; simpl in *; unfold shift_vwo in *;
 try (destruct v; inversion H0; subst);
 constructor; auto; omega.
@@ -304,16 +306,17 @@ try (rewrite IHN1; try rewrite IHN2; auto); auto.
 Qed.
 
 (* FIXME: Move this to Hybrid/Hyb_Substitution *)
-Lemma subst_w_Hyb_comm2:
-forall M w w' m n
-  (Neq: m <> n),
-  {{fwo w'//bwo m }}({{fwo w//bwo n}}M) =
-  {{fwo w//bwo n}}({{fwo w'//bwo m}}M).
-induction M; intros; simpl;
-repeat case_if; subst; simpl; auto;
-rewrite IHM || (rewrite IHM1; try rewrite IHM2);
-auto.
+Lemma subst_w_Hyb_shift_term_Hyb:
+forall M w w',
+  {{shift_vwo w // shift_vwo w'}} (shift_term_Hyb M) =
+  shift_term_Hyb ({{w//w'}}M).
+induction M; intros; destruct w; destruct w'; try destruct v;
+simpl in *; repeat case_if;
+try erewrite <- IHM;
+try erewrite <- IHM1; try erewrite <- IHM2; eauto.
 Qed.
+
+(* Term conversion *)
 
 Inductive L_to_Hyb_term: vwo -> te_L -> te_Hyb -> Prop :=
 | hyp_L_Hyb:
@@ -345,135 +348,168 @@ Inductive L_to_Hyb_term: vwo -> te_L -> te_Hyb -> Prop :=
       L_to_Hyb_term (shift_vwo w) M2 N2 ->
       L_to_Hyb_term w (letd_L M1 M2) (letdia_get_Hyb w N1 N2)
 | fetch_L_Hyb:
-    forall L M N w w',
-      (forall w0, w0 \notin L -> L_to_Hyb_term w M
-                                   (N ^w^ (fwo w0)))->
+    forall M N w w',
+      (* w <> w' -> (* no fetch in place! *) *)
+      L_to_Hyb_term w M N ->
       L_to_Hyb_term w' (fetch_L w M)
-                       (box_Hyb (unbox_fetch_Hyb (shift_vwo w)
-                                                 (shift_term_Hyb N)))
-| get_L_Hyb:
+                    (box_Hyb (unbox_fetch_Hyb (shift_vwo w) (shift_term_Hyb N)))
+| get_L_Hyb: (* ? *)
     forall M N w w',
       L_to_Hyb_term w M N ->
-      L_to_Hyb_term w'
-        (get_L w M)
-        (letdia_get_Hyb w N
-                        (get_here_Hyb (bwo 0)
-                                      (hyp_Hyb (bte 0))))
+      L_to_Hyb_term w' (get_L w M) N
 .
 
-Lemma L_to_Hyb_term_subst_w:
-forall M N w,
-  L_to_Hyb_term w M N ->
-  forall w0 n w',
-    (w' = if eq_vwo_dec w (bwo n) then (fwo w0) else w) ->
-    L_to_Hyb_term w' (subst_w_L M (fwo w0) (bwo n))
-                     (subst_w_Hyb (fwo w0) (bwo n) N).
-intros M N w H; induction H; intros; simpl in *; repeat case_if;
-simpl in *; try subst; eauto using L_to_Hyb_term.
-constructor; eapply IHL_to_Hyb_term; eauto; case_if; auto.
-constructor; eapply IHL_to_Hyb_term; eauto; case_if; auto.
-constructor; [eapply IHL_to_Hyb_term1 | eapply IHL_to_Hyb_term2];
-try case_if; auto.
-constructor; [eapply IHL_to_Hyb_term1 | eapply IHL_to_Hyb_term2];
-try case_if; auto.
-apply box_L_Hyb with (L:=L \u \{w0});
-intros; apply H0 with (w0:=w1); eauto; case_if; eauto; simpl in *;
-inversion H2; subst; repeat rewrite notin_union in H1;
-destruct H1 as (a, (b, c)); rewrite notin_singleton in c; elim c; auto.
-apply box_L_Hyb with (L:=L \u \{w0});
-intros; apply H0 with (w0:=w1); eauto; case_if; eauto; simpl in *;
-inversion H3; subst; repeat rewrite notin_union in H1;
-destruct H1 as (a, (b, c)); rewrite notin_singleton in c; elim c; auto.
-constructor; eapply IHL_to_Hyb_term; eauto; case_if; auto.
-constructor; eapply IHL_to_Hyb_term; eauto; case_if; auto.
-constructor; eapply IHL_to_Hyb_term; eauto; case_if; auto.
-constructor; eapply IHL_to_Hyb_term; eauto; case_if; auto.
-constructor; [eapply IHL_to_Hyb_term1 | eapply IHL_to_Hyb_term2];
-try case_if; auto.
-constructor; [eapply IHL_to_Hyb_term1 | eapply IHL_to_Hyb_term2];
-try case_if; auto; destruct w; simpl in *; inversion H1;
-subst; elim H2; auto.
-replace (bwo (S n)) with (shift_vwo (bwo n)) by (simpl; auto).
+Lemma test_fetch:
+forall w0 w1 w2 v M N,
+  M = fetch_L (fwo w0) (box_L (fetch_L (bwo 0)
+                                   (fetch_L (fwo w1) (hyp_L (fte v))))) ->
+  N = box_Hyb (unbox_fetch_Hyb (fwo w0) (box_Hyb (box_Hyb
+                                        (unbox_fetch_Hyb (bwo 2)
+                                        (box_Hyb (unbox_fetch_Hyb (fwo w1)
+                                                   (hyp_Hyb (fte v)))))))) ->
+  L_to_Hyb_term (fwo w2) M N.
+intros; subst;
 replace (fwo w0) with (shift_vwo (fwo w0)) by (simpl; auto).
-rewrite shift_vwo_shift_term_Hyb. simpl.
-apply fetch_L_Hyb with (L:=L \u \{w0});
-intros; unfold open_w_Hyb in *.
-destruct n; simpl in *.
-assert ({{fwo w1 // bwo 0}}({{fwo w0 // bwo 0}}N) = {{fwo w0 // bwo 0}}N).
-skip.
-rewrite H3. eapply H0.
-rewrite <- subst_w_Hyb_comm2; eauto.
-eapply H0; try case_if; auto.
-apply fetch_L_Hyb with (L:=L \u \{w0} \u \{w1});
-intros; unfold open_w_Hyb in *;
-rewrite <- subst_w_Hyb_comm; eauto;
-eapply H0; try case_if; auto.
-elim H2; auto.
-elim H2; auto.
-destruct w; simpl in *; inversion H3; subst; contradiction.
-destruct w; simpl in *; inversion H3; subst; contradiction.
-apply fetch_L_Hyb with (L:=L \u \{w0} \u \{w1});
-intros; unfold open_w_Hyb in *;
-rewrite <- subst_w_Hyb_comm; eauto;
-eapply H0; try case_if; auto.
-apply fetch_L_Hyb with (L:=L \u \{w0} \u \{w1});
-intros; unfold open_w_Hyb in *;
-rewrite <- subst_w_Hyb_comm; eauto;
-eapply H0; try case_if; auto.
-constructor; eapply IHL_to_Hyb_term; case_if; eauto.
-constructor; eapply IHL_to_Hyb_term; case_if; eauto.
-constructor; eapply IHL_to_Hyb_term; case_if; eauto.
-constructor; eapply IHL_to_Hyb_term; case_if; eauto.
-Qed.
+remember (box_Hyb (
+                                     unbox_fetch_Hyb (shift_vwo (fwo w1))
+                                           (shift_term_Hyb (hyp_Hyb (fte v)))
+                                         )) as M0.
+replace (box_Hyb
+              (box_Hyb
+                 (unbox_fetch_Hyb (bwo 2)
+                    (box_Hyb (unbox_fetch_Hyb (fwo w1) (hyp_Hyb (fte v)))))))
+        with (shift_term_Hyb (box_Hyb
+                                (box_Hyb (unbox_fetch_Hyb (shift_vwo (bwo 0))
+                                 (shift_term_Hyb M0)
+                                 ) ))).
+subst; econstructor; intros. unfold open_w_Hyb in *; repeat case_if.
+repeat econstructor.
 (*
-intros M N w H; induction H; intros; case_if; subst; simpl in *; repeat case_if;
-try (constructor; eapply IHL_to_Hyb_term; case_if; auto);
-try (constructor; [eapply IHL_to_Hyb_term1 | eapply IHL_to_Hyb_term2];
-     case_if; auto).
-apply box_L_Hyb with (L:=L \u var_from_vwo w0 \u var_from_vwo w1);
-intros; apply H0 with (w0:=w2); eauto; case_if; eauto;
-destruct w1; destruct w0; simpl in *;
-inversion H2; subst; repeat rewrite notin_union in H1;
-destruct H1 as (a, (b, c)); rewrite notin_singleton in c; elim c; auto.
-apply box_L_Hyb with (L:=L \u var_from_vwo w0 \u var_from_vwo w1);
-intros; apply H0 with (w0:=w2); eauto; case_if; eauto;
-destruct w1; destruct w0; simpl in *;
-inversion H3; subst; repeat rewrite notin_union in H1;
-destruct H1 as (a, (b, c)); rewrite notin_singleton in c; elim c; auto.
-destruct w1; destruct w; simpl in *; inversion H3; subst; try (elim H1; auto).
-unfold open_w_Hyb in *.
-(*
-rewrite shift_vwo_shift_term_Hyb; constructor; eapply IHL_to_Hyb_term;
-case_if; eauto.
-destruct w; destruct w1; simpl in *; inversion H1; subst; elim H0; auto.
-rewrite shift_vwo_shift_term_Hyb; constructor; eapply IHL_to_Hyb_term;
-case_if; eauto.
-rewrite shift_vwo_shift_term_Hyb; constructor; eapply IHL_to_Hyb_term;
-case_if; eauto.
-destruct w; destruct w1; simpl in *; inversion H2; subst; elim H0; auto.
-rewrite shift_vwo_shift_term_Hyb; constructor; eapply IHL_to_Hyb_term;
-case_if; eauto.
-destruct w1; simpl in *; inversion H0.
-destruct w1; simpl in *; inversion H1.
-destruct w1; simpl in *; inversion H0.
-destruct w1; simpl in *; inversion H2.
-Qed.
-*) *)
+econstructor. repeat case_if. simpl. intros.
+replace (box_Hyb
+              (unbox_fetch_Hyb
+                 (if eq_vwo_dec (fwo w1) (bwo 3) then fwo w3 else fwo w1)
+                 (hyp_Hyb (fte v)))) with
+    (shift_term_Hyb (box_Hyb
+              (unbox_fetch_Hyb
+                 (if eq_vwo_dec (fwo w1) (bwo 2) then fwo w3 else fwo w1)
+                 (hyp_Hyb (fte v))))).
+econstructor; intros. case_if.
+unfold open_w_Hyb; simpl; case_if. replace (hyp_Hyb (fte v)) with
+                                   (shift_term_Hyb (hyp_Hyb (fte v))).
+econstructor; intros. unfold open_w_Hyb; simpl; constructor.
+simpl; auto.
+simpl; repeat case_if; simpl; auto.
+*)
+subst; simpl; repeat case_if; simpl; auto.
+Grab Existential Variables.
+exact \{}.  (*exact \{}. exact \{}. exact \{}.  *)Qed.
 
-Lemma L_to_Hyb_term_subst_t:
-forall M N w C1 C2 v,
-  L_to_Hyb_term w M N -> lc_w_Hyb C2 ->
-  (forall w0, L_to_Hyb_term w0 C1 C2) ->
-  L_to_Hyb_term w (subst_t_L C1 v M) (subst_t_Hyb C2 v N).
-induction M; intros; inversion H; subst; simpl in *; try case_if;
-auto; try constructor; auto.
-apply box_L_Hyb with (L:=L); intros; apply IHM; auto.
-unfold shift_vte in *; destruct v0; [inversion H2 | discriminate].
-apply fetch_L_Hyb with (L:=L); intros;
-unfold open_w_Hyb in *; simpl in *.
-rewrite <- subst_Hyb_order_irrelevant_bound.
-eapply IHM; auto.
+Lemma test_fetch2:
+forall w0 w1 w2 v M N Omega Gamma G Gamma' A,
+  M = fetch_L (fwo w0) (box_L (fetch_L (bwo 0)
+                                   (fetch_L (fwo w1) (hyp_L (fte v))))) ->
+   N = box_Hyb (unbox_fetch_Hyb (fwo w0) (box_Hyb (box_Hyb
+                                        (unbox_fetch_Hyb (bwo 2)
+                                        (box_Hyb (unbox_fetch_Hyb (fwo w1)
+                                                   (hyp_Hyb (fte v)))))))) ->
+  w0 <> w1 -> w1 <> w2 -> w0 <> w2 ->
+   Omega; Gamma |- M ::: [*] [*] A @ w2 ->
+   Omega = w0 :: w1 :: w2 :: nil -> Gamma = (w1, (v, [*]A)) :: nil->
+   L_to_Hyb_ctx Omega Gamma w2 = (G, Some (w2, Gamma')) ->
+   G |= (w2, Gamma') |- N ::: [*] [*] A.
+intros.
+assert (L_to_Hyb_term (fwo w2) M N).
+eapply test_fetch; eauto.
+subst.
+unfold L_to_Hyb_ctx in *; simpl in *; repeat case_if; simpl in *;
+inversion H7; subst. clear H7.
+inversion H4; inversion HT; subst.
+unfold open_w_L in *; simpl in *; repeat case_if.
+apply t_box_Hyb with (L:=L).
+rew_app; repeat constructor; auto.
+  rewrite Mem_nil_eq; auto.
+  rewrite Mem_cons_eq; auto; intro nn; destruct nn; subst;
+  [elim H0 | rewrite Mem_nil_eq in *]; auto.
+  rewrite Mem_cons_eq; auto; intro nn; destruct nn; subst;
+  [elim H2 | rewrite Mem_cons_eq in *]; auto;
+  destruct H7; subst; [elim H3 | rewrite Mem_nil_eq in *]; auto.
+  rewrite Mem_nil_eq; auto.
+intros; unfold open_w_Hyb; simpl; repeat case_if.
+apply t_unbox_fetch_Hyb with (G:=(w1,(v, [*]A)::nil) :: (w2, nil) :: nil)
+                               (Gamma:=nil).
+skip.
+apply t_box_Hyb with (L:=L).
+skip. intros.
+apply t_box_Hyb with (L:=L).
+skip. intros.
+unfold open_w_Hyb; simpl; repeat case_if.
+rew_app.
+apply t_unbox_fetch_Hyb with (G:=(w0, nil)::(w2, nil)::
+                                 (w1, ((v, [*]A)::nil))::(w'0, nil)::nil)
+                             (Gamma:=nil).
+skip.
+apply t_box_Hyb with (L:=L).
+skip. intros.
+unfold open_w_Hyb; simpl; case_if.
+specialize HT0 with w'1. apply HT0 in H12. inversion H12. inversion HT1; subst.
+inversion HT2; subst.
+apply t_unbox_fetch_Hyb with (G:= (w2, nil) :: (w0, nil) ::
+                                            (w'0, nil) ::
+                                            (w'1, nil) :: (w', nil) :: nil)
+                               (Gamma:=(v, [*]A):: nil).
+skip.
+constructor. skip. apply Mem_here.
+PPermut_Hyb_simpl.
+PPermut_Hyb_simpl.
+PPermut_Hyb_simpl.
+Qed.
+
+(* FIXME: Move this to Labeled/Lists/L_Substitution *)
+Lemma lc_w_n_L_subst_t:
+forall N M v n,
+lc_w_n_L n (subst_t_L M v N) ->
+lc_w_n_L n N.
+induction N; intros; simpl in *; try destruct v; constructor;
+inversion H; subst; try eapply IHN; eauto.
+Qed.
+
+(* FIXME: Move this to Labeled/Lists/L_Substitution *)
+Lemma lc_w_n_L_subst_w:
+forall N w n,
+lc_w_n_L n (subst_w_L N (fwo w) (bwo n)) ->
+lc_w_n_L (S n) N.
+induction N; intros; simpl in *; try destruct v; constructor;
+inversion H; subst; try eapply IHN; eauto;
+repeat case_if; inversion H0; subst; try inversion H1; subst;
+try omega.
+Qed.
+
+(* FIXME: Move this to Labeled/Lists/L_Semantics *)
+Lemma types_L_lc_w_L:
+forall Omega Gamma M A w,
+  Omega; Gamma |- M ::: A @ w -> lc_w_L M.
+intros; induction H; constructor; try apply IHHT;
+unfold open_w_L in *; unfold open_t_L in *;
 auto.
+assert (exists x, x \notin L) by apply Fresh; destruct H0;
+specialize H with x; apply H in H0; apply lc_w_n_L_subst_t in H0; auto.
+assert (exists x, x \notin L) by apply Fresh; destruct H0;
+specialize H with x; apply H in H0; apply lc_w_n_L_subst_w in H0; auto.
+assert (exists x, x \notin Lt) by apply Fresh; destruct H1;
+assert (exists x, x \notin Lw) by apply Fresh; destruct H2;
+specialize H0 with x x0; apply H0 with (w':=x0) in H1; auto.
+apply lc_w_n_L_subst_t in H1; apply lc_w_n_L_subst_w in H1; auto.
+Qed.
+
+(* FIXME: Move this to Labeled/Lists/L_Semantics *)
+Lemma types_L_Mem_Omega:
+forall M Omega Gamma A w,
+  Omega; Gamma |- M ::: A @ w ->
+  Mem w Omega.
+intros; induction H; eauto;
+assert (exists x, x \notin L) as H0 by apply Fresh; destruct H0 as (x);
+apply H with (x:=x); auto.
 Qed.
 
 (* FIXME: Move this to Labeled/Lists/L_Substitution *)
@@ -512,27 +548,203 @@ destruct (eq_nat_dec m k); subst; [elim H0 |]; auto; omega.
 destruct (eq_nat_dec m k); subst; [elim H0 |]; auto; omega.
 Qed.
 
-(* FIXME: Move this to Labeled/Lists/L_Semantics *)
-Lemma types_L_Mem_Omega:
-forall M Omega Gamma A w,
-  Omega; Gamma |- M ::: A @ w ->
-  Mem w Omega.
-intros; induction H; eauto;
-assert (exists x, x \notin L) as H0 by apply Fresh; destruct H0 as (x);
-apply H with (x:=x); auto.
+(* FIXME: Move this to Hybrid/Hyb_Substitution *)
+Lemma lc_w_subst_Hyb_same_n_fwo:
+forall M w w' n,
+  lc_w_n_Hyb n M ->
+  lc_w_n_Hyb n {{fwo w // w'}} M.
+induction M; intros; simpl in *; repeat case_if;
+inversion H; subst; try destruct w;
+constructor; eauto.
 Qed.
 
-Lemma gather_keys_L_fresh:
-forall l w,
-  ~ Mem w (map fst l) ->
-  gather_keys_L w l = nil.
-induction l; intros; rew_map in *; simpl in *; auto.
-destruct a; case_if; simpl in *.
-elim H; apply Mem_here.
-rewrite IHl; auto; intro; elim H; rewrite Mem_cons_eq; right; auto.
+(* FIXME: Move this to Hybrid/Hyb_Substitution *)
+Lemma lc_w_subst_Hyb_same_n_bwo:
+forall M w' k n,
+  lc_w_n_Hyb n M ->
+  k < n ->
+  lc_w_n_Hyb n {{bwo k // w'}} M.
+induction M; intros; simpl in *; repeat case_if;
+inversion H; subst; try destruct w'; simpl;
+constructor; try (eapply IHM || eapply IHM2); try omega; auto.
 Qed.
 
-(* FIXME: do we really need all the 'locally closed' assumptions? *)
+(* FIXME: Move this to Hybrid/Hyb_Substitution *)
+Lemma subst_w_Hyb_comm2:
+forall M w w' m n
+  (Neq: m <> n)
+  (Neq': w <> bwo m),
+  {{fwo w'//bwo m }}({{w//bwo n}}M) =
+  {{w//bwo n}}({{fwo w'//bwo m}}M).
+induction M; intros; simpl; destruct w;
+repeat case_if; subst; simpl; auto;
+rewrite IHM || (rewrite IHM1; try rewrite IHM2);
+auto; intro nn; elim Neq'; inversion nn; subst; auto.
+Qed.
+
+(* FIXME: Move this to Hybrid/Hyb_Substitution *)
+Lemma double_subst_w_Hyb_bwo:
+forall N w w' n,
+ w' <> bwo n ->
+ {{w // bwo n}}({{w' // bwo n}}N) = {{w' // bwo n}}N.
+induction N; destruct w'; simpl in *; intros; repeat case_if;
+try rewrite IHN;
+try (rewrite IHN1; try rewrite IHN2); auto; intro nn; inversion nn;
+subst; elim H; auto.
+Qed.
+
+(* FIXME: Move this to Hybrid/Hyb_Substitution *)
+Lemma double_subst_w_Hyb_eq:
+forall M w0 n m,
+  subst_w_Hyb w0 (bwo n) (subst_w_Hyb (bwo n) (bwo m) M) =
+  subst_w_Hyb w0 (bwo n) (subst_w_Hyb w0 (bwo m) M).
+induction M; intros; simpl; repeat case_if;
+try rewrite IHM;
+try rewrite IHM1; try rewrite IHM2; eauto.
+Qed.
+
+(* FIXME: Move this to Hybrid/Hyb_Substitution *)
+Lemma reorder_subst_w_Hyb_eq:
+forall M w w' w'',
+  subst_w_Hyb w w' (subst_w_Hyb w w'' M) =
+  subst_w_Hyb w w'' (subst_w_Hyb w w' M).
+induction M; intros; simpl; repeat case_if;
+try rewrite IHM;
+try rewrite IHM1; try rewrite IHM2; eauto.
+Qed.
+
+Lemma L_to_Hyb_lc_w:
+forall M n,
+  lc_w_n_L n M ->
+  forall w N w' k,
+    (w = fwo w' \/ (w = bwo k /\ k < n)) ->
+    L_to_Hyb_term w M N -> lc_w_n_Hyb n N.
+induction M; intros; inversion H; inversion H1; subst;
+unfold open_w_Hyb in *.
+constructor.
+constructor; eapply IHM; eauto.
+constructor; [eapply IHM1 | eapply IHM2]; eauto.
+(* box *)
+constructor; assert (exists w0, w0 \notin L) by (apply Fresh);
+destruct H2 as (w0); apply IHM with (w:=fwo w0) (w':=w0) (k:=0); eauto.
+(* unbox_fetch *)
+destruct w.
+destruct H0; [ | destruct H0]; inversion H0; subst;
+constructor; try omega; eapply IHM; eauto.
+constructor; eapply IHM; eauto.
+(* get fwo *)
+destruct H0; [| destruct H0; inversion H0]; subst;
+eapply IHM with (n:=n) in H10; auto.
+(* get bwo *)
+destruct H0; [| destruct H0; inversion H0]; subst;
+eapply IHM with (n:=n) in H11; auto.
+(* letd *)
+destruct H0; [ | destruct H0; inversion H0]; subst; simpl in *.
+apply IHM1 with (n:=n) (w':=w') (k:=0) in H10; auto;
+apply IHM2 with (n:=S n) (w':=w') (k:=0) in H12; auto;
+constructor; auto.
+apply IHM1 with (n:=n) (w':=w') (k:=k) in H10; auto;
+apply IHM2 with (n:=S n) (w':=w') (k:=S k) in H12; auto;
+[constructor; auto | right; split; auto; omega].
+(* here *)
+destruct H0; [| destruct H0; inversion H0]; subst; constructor;
+try omega; eapply IHM; eauto.
+(* fetch fwo *)
+constructor; constructor;
+apply IHM with (w:=fwo w0)(N:=N0)(w':=w0)(k:=n) in H4; auto.
+apply lc_w_n_shift_term_Sn_Hyb; auto.
+(*apply closed_w_succ; auto.*)
+(* fetch bwo *)
+constructor; constructor; try omega;
+apply IHM with (w:=bwo m)(N:=N0)(w':=w')(k:=m) in H5;
+auto; try omega.
+apply lc_w_n_shift_term_Sn_Hyb; auto.
+(*apply closed_w_succ; auto.*)
+Grab Existential Variables.
+auto. auto. auto. auto. auto. auto. auto.
+Qed.
+
+Lemma L_to_Hyb_term_subst_t:
+forall M N w C1 C2 v,
+  L_to_Hyb_term w M N ->
+  lc_w_Hyb C2 -> shift_term_Hyb C2 = C2 ->
+  (forall w0, L_to_Hyb_term w0 C1 C2) ->
+  L_to_Hyb_term w (subst_t_L C1 v M) (subst_t_Hyb C2 v N).
+induction M; intros; inversion H; simpl in *; try case_if;
+auto; try constructor; auto;
+unfold open_w_L in *; unfold open_w_Hyb in *.
+apply box_L_Hyb with (L:=L); intros; apply IHM; auto.
+replace C2 with (shift_term_Hyb C2); auto.
+rewrite subst_t_Hyb_shift_term_Hyb; [constructor |]; auto.
+(*rewrite <- subst_t_Hyb_shift_term_Hyb; auto. apply IHM.
+auto. rewrite H1; auto. rewrite H1; auto. intros; rewrite H1; auto.*)
+Qed.
+
+Lemma L_to_Hyb_term_subst_w:
+forall M N w,
+  L_to_Hyb_term w M N ->
+  forall w0 w1 w',
+    (w' = if eq_vwo_dec w w0 then w1 else w) ->
+    L_to_Hyb_term w' (subst_w_L M w1 w0)
+                     (subst_w_Hyb w1 w0 N).
+intros; generalize dependent w0; generalize dependent w1;
+generalize dependent w'; induction H; intros; repeat case_if;
+simpl in *; repeat case_if; subst; eauto using L_to_Hyb_term;
+try (constructor; eapply IHL_to_Hyb_term; repeat case_if; eauto);
+try (constructor; [eapply IHL_to_Hyb_term1 | eapply IHL_to_Hyb_term2];
+     repeat case_if; eauto).
+
+apply box_L_Hyb with (L:=L \u var_from_vwo w0 \u var_from_vwo w1); intros;
+eapply H0; repeat case_if; eauto.
+repeat rewrite notin_union in H2; eauto; destruct H2; eauto.
+subst; destruct w0; simpl in *; inversion H2; subst;
+repeat rewrite notin_union in H1; eauto; destruct H1; destruct H3;
+apply notin_singleton in H3; elim H3; auto.
+
+apply box_L_Hyb with (L:=L \u var_from_vwo w0 \u var_from_vwo w1); intros;
+eapply H0; repeat case_if; eauto.
+repeat rewrite notin_union in H1; eauto; destruct H1; eauto.
+subst; destruct w0; simpl in *; inversion H3; subst;
+repeat rewrite notin_union in H1; eauto; destruct H1; destruct H4;
+apply notin_singleton in H4; elim H4; auto.
+
+destruct w; destruct w0; simpl in *; inversion H1; subst; elim H2; auto.
+
+rewrite subst_w_Hyb_shift_term_Hyb; constructor;
+(*rewrite <- subst_w_Hyb_shift_term_Hyb.*)
+eapply IHL_to_Hyb_term; case_if; auto.
+(* apply fetch_L_Hyb.*)
+
+destruct w; destruct w0; simpl in *; inversion H2; subst; elim H1; auto.
+
+rewrite subst_w_Hyb_shift_term_Hyb; constructor;
+eapply IHL_to_Hyb_term; case_if; auto.
+
+rewrite subst_w_Hyb_shift_term_Hyb; constructor;
+eapply IHL_to_Hyb_term; case_if; auto.
+
+destruct w; destruct w0; simpl in *; inversion H3; subst; elim H2; auto.
+
+rewrite subst_w_Hyb_shift_term_Hyb; constructor;
+eapply IHL_to_Hyb_term; case_if; auto.
+Qed.
+
+Lemma types_Hyb_shift_term:
+forall M G Gamma w A,
+  G |= (w, Gamma) |- M ::: A ->
+  G |= (w, Gamma) |- shift_term_Hyb M ::: A.
+intros; induction H; simpl in *; eauto using types_Hyb;
+unfold open_w_Hyb in *; unfold open_t_Hyb in *.
+econstructor; eauto; intros; unfold open_t_Hyb in *;
+replace (hyp_Hyb (fte v')) with (shift_term_Hyb (hyp_Hyb (fte v')))
+                                  by (simpl; auto);
+rewrite subst_t_Hyb_shift_term_Hyb; eauto; constructor.
+econstructor; eauto; intros; unfold open_w_Hyb.
+specialize H with w'; apply H in H0;
+rewrite <- subst_w_Hyb_shift_term_Hyb in H0; simpl in *.
+replace ({{fwo w' // bwo 0}}(shift_term_Hyb M)) with (shift_term_Hyb M).
+Admitted.
+
 Lemma L_to_Hyb_typing:
 forall Omega_L Gamma_L M_L A w_L G_Hyb Gamma_Hyb M_Hyb,
   L_to_Hyb_ctx Omega_L Gamma_L w_L = (G_Hyb, Some (w_L, Gamma_Hyb)) ->
@@ -544,26 +756,29 @@ unfold L_to_Hyb_ctx; intros;
 generalize dependent G_Hyb;
 generalize dependent Gamma_Hyb;
 generalize dependent M_Hyb;
-induction H3; intros; inversion H0; subst; simpl in *;
-inversion H1; inversion H2; subst.
+induction H3; intros; inversion H0; subst; simpl in *.
 (* hyp *)
 constructor;
 [apply ok_L_to_Hyb_ctx_ok_Hyb with (Omega:=Omega) (Gamma:=Gamma) (w:=w)| ];
 auto; eapply Mem_L_to_Hyb_ctx; eauto.
 (* lam *)
+inversion H1; inversion H2; subst.
 apply t_lam_Hyb with (L:=L);
 [eapply ok_L_to_Hyb_ctx_ok_Hyb; eauto | intros]; unfold open_t_Hyb in *;
 unfold open_t_L in *; apply H with (x:=v'); auto.
 apply lc_w_subst_t_L; [constructor | ]; auto.
 apply L_to_Hyb_term_subst_t; simpl; auto.
-constructor. intros; constructor.
+constructor.
+intros; constructor.
 apply lc_w_subst_t_Hyb; [constructor | ]; auto.
 destruct Ok; apply split_at_Hyb_cons; auto.
 (* appl *)
+inversion H1; inversion H2; subst;
 apply t_appl_Hyb with (A:=A);
 [eapply ok_L_to_Hyb_ctx_ok_Hyb |
  apply IHtypes_L1 | apply IHtypes_L2]; eauto.
 (* box *)
+inversion H1; inversion H2; subst;
 apply t_box_Hyb with (L:=L \u L0 \u
                            from_list (map fst Gamma)).
 assert (G_Hyb & (w, Gamma_Hyb) ~=~ (w, Gamma_Hyb) :: G_Hyb) as HP
@@ -582,26 +797,97 @@ apply lc_w_subst_Hyb; auto.
 case_if; destruct Ok.
 rewrite gather_keys_L_fresh; [|apply notin_Mem]; eauto.
 (* unbox *)
+inversion H1; inversion H2; subst;
 apply t_unbox_Hyb; auto;
 eapply ok_L_to_Hyb_ctx_ok_Hyb; eauto.
 (* fetch *)
-apply t_box_Hyb with (L:=L \u used_w_vars_Hyb ((w', Gamma_Hyb) :: G_Hyb)).
-assert (G_Hyb & (w', Gamma_Hyb) ~=~ (w', Gamma_Hyb) :: G_Hyb)
-  by PPermut_Hyb_simpl; rewrite H4;
+apply t_box_Hyb with (L:=used_w_vars_Hyb ((w', Gamma_Hyb) :: G_Hyb)).
+assert (G_Hyb & (w', Gamma_Hyb) ~=~ (w', Gamma_Hyb) :: G_Hyb) as HP
+  by PPermut_Hyb_simpl; rewrite HP;
 eapply ok_L_to_Hyb_ctx_ok_Hyb; eauto.
-intros; unfold open_w_L in *; unfold open_w_Hyb in *; simpl;
+intros; unfold open_w_Hyb; simpl; case_if;
+destruct (eq_var_dec w w').
+(* = *)
+subst.
+apply t_unbox_fetch_Hyb with (G:=G_Hyb) (Gamma:=Gamma_Hyb); auto.
+assert ((w', Gamma_Hyb) :: G_Hyb & (w'0, nil) ~=~
+        (w'0, nil) :: (w', Gamma_Hyb) :: G_Hyb) by PPermut_Hyb_simpl;
+rewrite H6; apply ok_Bg_Hyb_fresh_wo; [eapply ok_L_to_Hyb_ctx_ok_Hyb | ]; eauto.
+assert (G_Hyb & (w'0, nil) ~=~ nil & (w'0, nil) ++ G_Hyb) by PPermut_Hyb_simpl;
+rewrite H6; apply GlobalWeakening_Hyb; rew_app;
+inversion H2; inversion H10; inversion H1; subst.
+Focus 2.
+assert ((w', Gamma_Hyb) :: (w'0, nil) :: G_Hyb ~=~
+        (w'0, nil) :: (w', Gamma_Hyb) :: G_Hyb) by PPermut_Hyb_simpl;
+rewrite H7; apply ok_Bg_Hyb_fresh_wo; [eapply ok_L_to_Hyb_ctx_ok_Hyb | ]; eauto.
+apply IHtypes_L with (M_Hyb:=N) (Gamma_Hyb:=Gamma_Hyb)(G_Hyb:=G_Hyb) in H17;
+auto.
+Focus 2.
+apply lc_w_n_shift_term_Sn_Hyb; auto.
+assert (lc_w_Hyb N). apply lc_w_n_shift_term_Sn_Hyb; auto.
+replace N with ({{fwo w'0 // bwo 0}}N) in H17.
+Focus 2. erewrite closed_subst_w_Hyb_bound; eauto.
+
+
+apply lc_w_subst_Hyb; auto.
+assert ((w', Gamma_Hyb) :: (w'0, nil) :: G_Hyb ~=~
+        (w'0, nil) :: (w', Gamma_Hyb) :: G_Hyb) by PPermut_Hyb_simpl;
+rewrite H9. apply ok_Bg_Hyb_fresh_wo; auto;
+eapply ok_L_to_Hyb_ctx_ok_Hyb; eauto.
+
+
+(* <> *)
+assert (exists Gw Gammaw, L_to_Hyb_ctx Omega Gamma w =
+                          (Gw, Some (w, Gammaw))).
+  exists (fst (split_at_Hyb (bucket_sort_L Omega Gamma) w)).
+  assert (exists Gamma1, snd (split_at_Hyb (bucket_sort_L Omega Gamma) w) =
+                 Some (w, Gamma1)).
+  apply L_to_Hyb_ctx_Mem_Some;  apply types_L_Mem_Omega in H3; auto.
+  destruct H5; exists x; rewrite <- H5; apply surjective_pairing.
+destruct H5 as (G_w, (Gamma_w, H5)).
+assert ((w', Gamma_Hyb) :: G_Hyb *=* (w, Gamma_w) :: G_w).
+  transitivity (bucket_sort_L Omega Gamma); [symmetry |];
+  unfold L_to_Hyb_ctx in *; apply bucket_sort_L_permut; auto.
+apply permut_split_head in H6; destruct H6 as (hd, (tl, H6)).
+
+assert (exists G0, G_Hyb ~=~ G0 & (w, Gamma_w)).
+
+
+skip. destruct H6 as (G0).
+rewrite H6. unfold open_w_Hyb in *; simpl.
 case_if.
+apply t_unbox_fetch_Hyb with (G:=G0&(w_L, Gamma_Hyb)) (Gamma:=Gamma_w).
+skip.
+specialize IHM_L with Omega_L Gamma_L ([*]A0) w G_w Gamma_w N.
+apply IHM_L in H5; auto.
+Focus 2. inversion H1; subst; auto. Focus 2. skip. (* from H15 + inv. H1 *)
+assert (G_w ~=~ G0 & (w_L, Gamma_Hyb)). skip.
+rewrite  H8 in H5.
+assert (lc_w_Hyb N). skip.
+rewrite closed_subst_w_Hyb_bound with (n:=0); auto.
+replace (G0 & (w_L, Gamma_Hyb) & (w', nil)) with
+ ((G0 & (w_L, Gamma_Hyb)) & (w', nil) ++ nil) by (rew_app; auto).
+apply GlobalWeakening_Hyb; rew_app; auto.
+skip. PPermut_Hyb_simpl.
+
+
+
 destruct (eq_var_dec w w'); subst.
 (* w = w' *)
+eapply IHtypes_L; auto.
+inversion H1; subst; auto.
+apply H8.
 apply t_unbox_fetch_Hyb with (G:=G_Hyb) (Gamma:=Gamma_Hyb); auto.
 assert ((w', Gamma_Hyb) :: G_Hyb & (w'0, nil) ~=~
         (w'0, nil) :: (w', Gamma_Hyb) :: G_Hyb) by PPermut_Hyb_simpl;
 rewrite H7; apply ok_Bg_Hyb_fresh_wo; [eapply ok_L_to_Hyb_ctx_ok_Hyb | ]; eauto.
-inversion H11; subst.
 assert (G_Hyb & (w'0, nil) ~=~ nil & (w'0, nil) ++ G_Hyb) by PPermut_Hyb_simpl.
 rewrite H7; apply GlobalWeakening_Hyb; rew_app.
+inversion
 eapply IHtypes_L; auto.
-(*apply lc_w_n_shift_term_Sn_Hyb in H10.
+rewrite H13.
+apply lc_w_n_shift_term_Sn_Hyb in H10.
+
 rewrite lc_w_shift_term_Hyb; auto;
 inversion H0; subst. apply H13; auto.
 rewrite closed_subst_w_Hyb_bound with (n:=0); auto. *)
@@ -613,6 +899,12 @@ eapply ok_L_to_Hyb_ctx_ok_Hyb; eauto.
 (* w <> w' *)
 assert (exists G0, exists Gamma0,
           split_at_Hyb (bucket_sort_L Omega Gamma) w = (G0, Some (w, Gamma0))).
+  exists (fst (split_at_Hyb (bucket_sort_L Omega Gamma) w)).
+  assert (exists Gamma1, snd (split_at_Hyb (bucket_sort_L Omega Gamma) w) =
+                 Some (w, Gamma1)).
+  apply L_to_Hyb_ctx_Mem_Some.
+  apply types_L_Mem_Omega in H3; auto.
+  destruct H7; exists x; rewrite <- H7; apply surjective_pairing.
   exists (fst (split_at_Hyb (bucket_sort_L Omega Gamma) w)).
   assert (exists Gamma1, snd (split_at_Hyb (bucket_sort_L Omega Gamma) w) =
                  Some (w, Gamma1)).
@@ -733,7 +1025,22 @@ rewrite gather_keys_L_fresh; [| apply notin_Mem]; eauto;
 symmetry in H4; rewrite surjective_pairing in H4; inversion H4; subst;
 rewrite H18; auto.
 Qed
-              .
+
+
+(*
+Lemma L_to_Hyb_typing_alt_formulation:
+forall Omega_L Gamma_L M_L A w_L G_Hyb Gamma_Hyb,
+  L_to_Hyb_ctx Omega_L Gamma_L w_L = (G_Hyb, Some (w_L, Gamma_Hyb)) ->
+  Omega_L; Gamma_L |- M_L ::: A @ w_L ->
+  exists M_Hyb,
+    L_to_Hyb_term (fwo w_L) M_L M_Hyb /\
+    G_Hyb |= (w_L, Gamma_Hyb) |- M_Hyb ::: A.
+intros. induction H0.
+exists (hyp_Hyb (fte v)); split; constructor; eauto;
+[ eapply ok_L_to_Hyb_ctx_ok_Hyb |
+  eapply Mem_L_to_Hyb_ctx]; eauto.
+*)
+     .
 
 Lemma L_to_Hyb_steps:
 forall M N w M',
@@ -750,3 +1057,7 @@ Admitted. (* problem for box *)
 Close Scope labeled_is5_scope.
 Close Scope permut_scope.
 Close Scope is5_scope.
+
+(*
+forall Omega Gamma M M ::: A , exists M' relation M M' /\ M' :: A
+*)
